InferFix.v
@@ -1,0 +1,77 @@
+Require Export SystemFR.ReducibilityLemmas.
+Require Export SystemFR.TypeSugar2.
+Require Export SystemFR.StepTactics.
+
+Lemma subst_fix_default:
+  forall t default fuel l tag,
+    wfs l 0 ->
+    psubstitute (fix_default t default fuel) l tag =
+    fix_default (psubstitute t l tag) (psubstitute default l tag) (psubstitute fuel l tag).
+Proof.
+  unfold fix_default; repeat step || t_equality || rewrite substitute_shift_open in *.
+Qed.
+
+Lemma evaluate_fix_default:
+  forall t default fuel,
+    is_nat_value fuel ->
+    wf default 0 ->
+    wf t 1 ->
+    (fuel = zero /\ star scbv_step (fix_default t default fuel) default) \/
+    (exists fuel', fuel = succ fuel' /\
+              star scbv_step (fix_default t default fuel) (open 0 t (fix_default t default fuel'))).
+Proof.
+  unfold fix_default; inversion 1; steps.
+  - left; steps.
+    one_step; repeat open_none.
+    repeat one_step.
+  - right; eexists; steps.
+    one_step; repeat open_none.
+    one_step.
+    one_step; repeat open_none_by ltac:(eauto 2 with wf step_tactic).
+
+    .
+    rewrite (open_none _ 3).
+    admit.
+    eauto with wf step_tactic.
+    apply wf_shift_open2; steps.
+    eauto with wf step_tactic.
+
+
+    wf_shift_open2
+
+    open_none.
+    rewrite open_none. in * by auto.
+    star_one_step
+  
+
+
+Opaque fix_default.
+
+Lemma tfix_fuel:
+  forall ρ t default fuel T,
+    is_nat_value fuel
+    [ ρ | default : T ] ->
+    (forall v, [ ρ | v : T ]v -> [ ρ | open 0 t v : T ]) ->
+    [ ρ | fix_default t default fuel : T ].
+Proof.
+Admitted.
+
+Lemma open_tfix_helper:
+  forall Θ Γ t default fuel x T,
+    [ Θ; Γ ⊨ fuel : T_nat ] ->
+    [ Θ; Γ ⊨ default : T ] ->
+    [ Θ; (x, T) :: Γ ⊨ open 0 t (fvar x term_var) : T ] ->
+    [ Θ; Γ ⊨ fix_default t default fuel : T ].
+Proof.
+  unfold open_reducible; steps.
+²Admitted.
+
+Lemma open_tfix:
+  forall Γ t default fuel x T,
+    [ Γ ⊨ fuel : T_nat ] ->
+    [ Γ ⊨ default : T ] ->
+    [ (x, T) :: Γ ⊨ open 0 t (fvar x term_var) : T ] ->
+    [ Γ ⊨ fix_default t default fuel : T ].
+Proof.
+  eauto using open_tfix_helper.
+Qed.
