StepTactics.v
@@ -1,0 +1,9 @@
+Require Export SystemFR.WFLemmas.
+Require Export SystemFR.SmallStep.
+Require Export SystemFR.RelationClosures.
+
+Ltac one_step_aux :=
+ eapply Trans; [ eauto using is_nat_value_build_nat with values smallstep cbvlemmas | idtac ];
+   repeat step || (rewrite open_none in * by (repeat step; eauto using is_nat_value_build_nat with wf)).
+
+Ltac one_step := unshelve one_step_aux; steps.
